Let's analyze the behavior of `append` and `append!` step by step, using box-and-pointer diagrams to visualize the list structures.

### 1. Initial Definitions
```scheme
(define x (list 'a 'b))  ; x → ['a, 'b]
(define y (list 'c 'd))  ; y → ['c, 'd]
```
Box-and-pointer diagrams:
```
x: [a|•] → [b|/]
y: [c|•] → [d|/]
```

### 2. Evaluating `(define z (append x y))`
The `append` procedure is a **non-mutating** version that constructs a new list by copying the elements of `x` and linking them to `y`:
```scheme
(define (append x y)
  (if (null? x)
      y
      (cons (car x) (append (cdr x) y))))
```
- `(append x y)` recursively copies `x` and links the last copied pair to `y`:
  - `(cons 'a (append '(b) '(c d)))` → `(cons 'a (cons 'b '(c d)))` → `'(a b c d)`.

Result:
```
z: [a|•] → [b|•] → [c|•] → [d|/]
```
- `x` remains unchanged: `(cdr x)` is still `'(b)`.
- `y` remains unchanged: `'(c d)`.

#### Missing Response for `(cdr x)`:
```scheme
(cdr x)  ; → (b)
```

### 3. Evaluating `(define w (append! x y))`
The `append!` procedure is a **mutating** version that modifies the last pair of `x` to point to `y`:
```scheme
(define (append! x y)
  (set-cdr! (last-pair x) y)
  x)
```
- `(last-pair x)` finds the last pair of `x`, which is `'(b)`.
- `(set-cdr! '(b) y)` modifies the cdr of `'(b)` to point to `y`.

Result:
```
x (and w): [a|•] → [b|•] → [c|•] → [d|/]
```
- Now `x` is mutated: `(cdr x)` is `'(b c d)`.
- `y` is now part of the mutated `x`.

#### Missing Response for `(cdr x)`:
```scheme
(cdr x)  ; → (b c d)
```

### Box-and-Pointer Diagrams
#### After `(define z (append x y))`:
```
x: [a|•] → [b|/]
y: [c|•] → [d|/]
z: [a|•] → [b|•] → [c|•] → [d|/]
```
- `z` is a new list, independent of `x` and `y`.

#### After `(define w (append! x y))`:
```
x (and w): [a|•] → [b|•] → [c|•] → [d|/]
y: [c|•] → [d|/]
```
- `x` is mutated, and `w` shares the same structure as `x`.
- `y` is now part of `x`'s structure.

### Final Answers:
1. After `(define z (append x y))`:
   ```scheme
   (cdr x)  ; → (b)
   ```
2. After `(define w (append! x y))`:
   ```scheme
   (cdr x)  ; → (b c d)
   ```

### Key Observations:
- `append` creates a **new list** without modifying `x` or `y`.
- `append!` **mutates** `x` by splicing `y` onto it, so `x` and `w` share the same structure afterward.
- `y` is now part of `x` after `append!`, so modifying `y` later would affect `x` (and `w`).